Core/Metatheory/Preservation/Lemmas.lean
@@ -1,0 +1,230 @@
+import LeanSubst
+import Core.Term
+import Core.Term.Spine
+import Core.Reduction
+import Core.Typing
+import Core.Util
+
+import Core.Metatheory.Rename
+import Core.Metatheory.Substitution
+import Core.Metatheory.GlobalWf
+import Core.Metatheory.Uniqueness
+import Core.Metatheory.Inversion
+import Core.Metatheory.SpineType
+
+open LeanSubst
+
+theorem instance_type_preservation :
+  ⊢ G ->
+  G&Δ, Γ ⊢ g#x : T ->
+  is = instances x G ->
+  ∀ t ∈ is, ∀ Δ Γ, G&Δ, Γ ⊢ t : T := by
+intro wf j h t t_in_is
+sorry
+
+theorem lookup_defn_type_sound :
+  ⊢ G ->
+  lookup x G = .some (Entry.defn y T t) ->
+  ∀ Δ Γ, G&Δ, Γ ⊢ t : T := by
+intro wf h
+induction G <;> simp [lookup] at *
+case _ hd tl ih =>
+  cases wf; case _ wfh wft =>
+  cases hd <;> simp [lookup] at *
+  case data =>
+    sorry
+  case opent => sorry
+  case openm => sorry
+  case defn => sorry
+  case inst => sorry
+  case instty =>
+    split at h
+    cases h
+    replace ih := ih wfh h
+    sorry -- need weakening on globals
+
+
+
+theorem Typing.foldr_preservation_choiceₗ :
+    G&Δ ⊢ B : .base b ->
+    G&Δ, Γ ⊢ a : B ->
+    (∀ t ∈ is,  G&Δ, Γ ⊢ t : B) ->
+    G&Δ, Γ ⊢ List.foldr (λ t acc => t `+ acc) a is : B := by
+intro h1 h2 h3 ; induction is using List.foldr.induct <;> simp at *
+assumption
+case _ ih =>
+  apply Typing.choice
+  apply h1;
+  apply h3.1
+  apply ih h3.2
+
+theorem Typing.foldr_preservation :
+  G&Δ ⊢ T : .base b ->
+  (∀ t ∈ is, G&Δ, Γ ⊢ t : T) ->
+  G&Δ, Γ ⊢ List.foldr (·`+·) `0 is : T := by
+intro j h
+induction is <;> simp at *
+constructor; assumption
+case _ hd tl ih =>
+  apply Typing.choice
+  apply j
+  apply h.1
+  apply ih h.2
+
+
+theorem fix_quantifiers {is : List Term} {Δ : List Kind} {Γ : List Ty} :
+  (∀ t ∈ is, ∀ Δ Γ, G&Δ, Γ ⊢ t : T) ->
+  (∀ t ∈ is, G&Δ, Γ ⊢ t : T) := by
+intro h
+intro t h1
+apply h t h1
+
+
+theorem preservation_prefix_match_lemma :
+  ⊢ G ->
+  a.spine = some (x, sp) ->
+  G&Δ,Γ ⊢ a : A ->
+  G&Δ,Γ ⊢ a.apply ξ : R ->
+  G&Δ,Γ ⊢ t : B ->
+  StableTypeMatch Δ A R -> -- R is the return type of A
+  PrefixTypeMatch Δ A B T -> -- T is B's return type and A and B have same prefixes
+  G&Δ,Γ ⊢ t.apply ξ : T := by
+intro wf h1 h2 h3 h4 h5 h6
+induction ξ generalizing G Δ Γ A R B T a t x sp
+case _ =>
+   simp [Term.apply] at *
+   have e := Typing.spine_term_unique_typing h2 h3 h1; cases e
+   have e := StableTypeMatch.prefix_type_match_forced_refl h5 h6; cases e
+   assumption
+case _ hd tl ih =>
+    have lem : (hd :: tl) = [hd] ++ tl := by simp
+    rw[lem, Spine.apply_spine_compose] at h3; rw[lem, Spine.apply_spine_compose]; clear lem
+    have lem := Typing.inversion_apply_spine wf h3
+    rcases lem with ⟨B', h1, h2, _, h3⟩
+    cases hd <;> simp [Term.apply] at *
+    case type hd =>
+      cases h5
+      case refl =>
+        cases h2; case _ e =>
+        -- subst e
+        replace ih := @ih G x sp Δ Γ (a •[hd]) B' A (t •[hd]) B T wf (sorry) (sorry) h3
+        sorry
+      case all => sorry
+      case arrow => sorry
+
+      -- replace ih := @ih G x sp Δ Γ (a •[hd]) B' R (t •[hd]) B T wf (sorry) h2 h3 sorry
+    case term hd =>
+      -- have lem := Typing.inversion_apply_spine wf h3
+      -- rcases lem with ⟨B', h1, h2, _, h3⟩
+      -- apply ih wf
+
+      -- have lem : StableTypeMatch Δ A (argA -:> R) := by apply StableTypeMatch.arrow; sorry
+      -- have ih1 := ih
+      sorry
+
+    case oterm hd => sorry
+
+-- apply @List.reverse_ind SpineElem
+--   (λ ξ => ∀ G Δ Γ A R B T a t, ∀ x: String,  ∀ (sp : List SpineElem),
+--     ⊢ G ->
+--     a.spine = some (x, sp) ->
+--     G&Δ,Γ ⊢ a : A ->
+--     G&Δ,Γ ⊢ a.apply ξ : R ->
+--     G&Δ,Γ ⊢ t : B ->
+--     StableTypeMatch Δ A R ->
+--     PrefixTypeMatch Δ A B T ->
+--     G&Δ,Γ ⊢ t.apply ξ : T)
+--   ξ
+--   (by
+--    intro G Δ Γ A R B T a t x sp wf h1 h2 h3 h4 h5 h6
+--    simp [Term.apply] at *
+--    have e := Typing.spine_term_unique_typing h2 h3 h1; cases e
+--    have e := StableTypeMatch.prefix_type_match_forced_refl h5 h6; cases e
+--    assumption)
+--   (by
+--     intro hd tl ih G Δ Γ A R B T a t x sp wf h1 h2 h3 h4 h5 h6
+--     rw[Spine.apply_spine_compose] at h3; rw[Spine.apply_spine_compose]
+--     cases hd
+--     case type =>
+--       cases h5 <;> simp [Term.apply] at *
+--       case refl =>
+--         cases h3; case _ h3 e =>
+--         replace h3 := Typing.inversion_apply_spine wf h3
+--         rcases h3 with ⟨w, j1, j2, _, j3⟩
+--         have lem := Typing.spine_term_unique_typing h2 j2 h1; subst lem
+--         sorry
+--       case arrow => sorry
+--       case all => sorry
+--     case term =>
+--       simp [Term.apply] at *
+--       cases h3; case _ X q1 q2 q3 =>
+--       replace h3 := Typing.inversion_apply_spine wf q3
+--       rcases h3 with ⟨w, j1, j2, _, j3⟩
+--       have lem := Typing.spine_term_unique_typing h2 j2 h1; subst lem
+--       have lem : PrefixTypeMatch Δ (X -:> A) (X -:> B) T := by
+--           apply PrefixTypeMatch.arrow; assumption
+--       have lem' : StableTypeMatch Δ (X -:> A) R := by
+--           apply StableTypeMatch.arrow; assumption
+
+--       cases h5
+--       case refl =>
+--         apply Typing.app
+--         apply q1
+--         apply ih (A := A) (R := X -:> R) (B := B) (T := X -:> T)
+--         · apply wf
+--         · apply h1
+--         · apply h2
+--         · sorry
+--         · apply h4
+--         · sorry
+--         · sorry
+
+--         apply q2
+--       case arrow =>
+--         apply Typing.app
+--         apply q1
+--         sorry
+--         apply q2
+--       case all => sorry
+
+--     case oterm => sorry
+
+
+
+    -- case type hd =>
+
+    --   sorry
+    -- case term hd =>
+    --   cases h3; case _ argA j1 j2 j3 =>
+    --   have lem := Typing.inversion_apply_spine wf j3
+    --   rcases lem with ⟨B', lem1, lem2, _, lem3⟩
+    --   -- have lem : StableTypeMatch Δ A (argA -:> R) := by apply StableTypeMatch.arrow; sorry
+
+    --   apply Typing.app
+    --   apply j1
+    --   sorry
+    --   apply j2
+    -- case oterm hd => sorry
+
+  -- )
+  -- G Δ Γ A R B T a t x sp wf h1 h2 h3 h4 h5 h6
+
+
+theorem preservation_prefix_match {p s t : Term} :
+  ⊢ G ->
+  G&Δ,Γ ⊢ p : A ->
+  G&Δ,Γ ⊢ s : R ->
+  G&Δ,Γ ⊢ t : B ->
+  StableTypeMatch Δ A R ->
+  PrefixTypeMatch Δ A B T ->
+  prefix_equal sp sp' = some ξ ->
+  p.spine = some (x, sp) ->
+  s.spine = some (x, sp') ->
+  G&Δ,Γ ⊢ t.apply ξ : T
+:= by
+intro wf j1 j2 j3 j4 j5 j6 j7 j8
+replace j6 := prefix_equal_law j6; subst j6
+have h7 := Spine.apply_eq j7; subst h7
+replace j8 := Spine.apply_eq j8; subst j8
+rw [Spine.apply_spine_compose] at j2
+apply preservation_prefix_match_lemma wf j7 j1 j2 j3 j4 j5
