Core/Metatheory/Progress.lean
@@ -3,4 +3,131 @@ import Core.Term
 import Core.Reduction
 import Core.Typing
 
-open LeanSubst
+import Core.Metatheory.ValueSoundness
+
+theorem progress_lemma :
+  ⊢ G ->
+  Γ = [] ->
+  G&Δ,Γ ⊢ t : T ->
+  Value G t ∨ t = `0 ∨ ∃ t', G ⊢ t ~> t' := by
+intro wf e j
+induction j
+case var => subst e; simp at *
+case global =>
+  subst e
+
+  sorry
+case mtch =>
+  subst e
+  sorry
+case guard =>
+  subst e
+  sorry
+case lam => apply Or.inl; apply Value.lam
+case lamt => apply Or.inl; apply Value.lamt
+case zero => apply Or.inr; apply Or.inl; rfl
+case refl => apply Or.inl; apply Value.refl
+case app b _ _ _ _ _ _ _ ih1 ih2 =>
+  cases b
+  case _ =>
+    cases ih2 e
+    case _ => sorry
+    case _ => sorry
+  case _ =>
+    sorry
+
+case appt => sorry
+case cast t A _ _ _ _ j _ ih =>
+  cases ih e
+  case _ h =>
+    have lem := refl_is_val j h
+    cases lem;
+    case _ lem =>
+      rcases lem with ⟨e1, e2⟩; subst e1; subst e2
+      apply Or.inr; apply Or.inr; exists t; apply Red.cast
+    case _ lem =>
+      rcases lem with ⟨c1, c2, e⟩; subst e
+      apply Or.inr; apply Or.inr
+      exists (t ▹ c1) `+  (t ▹ c2)
+      apply Red.ctor2_map2; simp; simp
+  case _ lem =>
+     cases lem
+     case _ h => subst h; apply Or.inr; apply Or.inr; exists `0; apply Red.ctor2_absorb2 (v := .cast); simp
+     case _ h =>
+       rcases h with ⟨c', h⟩
+       apply Or.inr; apply Or.inr; exists (t ▹ c')
+       apply Red.ctor2_congr2 (by simp) h
+
+case sym ih =>
+  cases ih e
+  case _ ih => sorry
+  case _ ih =>
+    cases ih
+    case _ ih => sorry
+    case _ ih => sorry
+
+case seq ih1 ih2 =>
+  cases ih1 e
+  case _ ih1 => sorry
+  case _ ih1 =>
+    cases ih1
+    case _ ih1 => sorry
+    case _ ih1 => sorry
+
+
+case appc ih1 ih2 =>
+  cases ih1 e
+  case _ ih1 => sorry
+  case _ ih1 =>
+    cases ih1
+    case _ ih1 => sorry
+    case _ ih1 => sorry
+
+case arrowc ih1 ih2 =>
+  cases ih1 e
+  case _ ih1 => sorry
+  case _ ih1 =>
+    cases ih1
+    case _ ih1 => sorry
+    case _ ih1 => sorry
+
+case fst ih1 =>
+  cases ih1 e
+  case _ ih1 => sorry
+  case _ ih1 =>
+    cases ih1
+    case _ ih1 => sorry
+    case _ ih1 => sorry
+
+case snd ih1 =>
+  cases ih1 e
+  case _ ih1 => sorry
+  case _ ih1 =>
+    cases ih1
+    case _ ih1 => sorry
+    case _ ih1 => sorry
+
+case allc Γ _ ih1 =>
+  have e' : List.map (λ x => x[+1]) Γ = [] := by rw[e]; simp
+  cases ih1 e'
+  case _ ih1 => sorry
+  case _ ih1 =>
+    cases ih1
+    case _ ih1 => sorry
+    case _ ih1 => sorry
+
+case apptc ih1 =>
+  cases ih1 e
+  case _ ih1 => sorry
+  case _ ih1 =>
+    cases ih1
+    case _ ih1 => sorry
+    case _ ih1 => sorry
+
+case choice ih1 ih2 =>
+  cases ih1 e
+  case _ ih1 => sorry
+  case _ ih1 =>
+    cases ih1
+    case _ ih1 => sorry
+    case _ ih1 => sorry
